# baseURI: urn:x-evn-master:movieontology

BASE   <urn:x-evn-master:movieontology>
PREFIX metadata: <http://topbraid.org/metadata#>
PREFIX teamwork: <http://topbraid.org/teamwork#>
PREFIX owl: <http://www.w3.org/2002/07/owl#>
PREFIX rdf: <http://www.w3.org/1999/02/22-rdf-syntax-ns#>
PREFIX sh: <http://www.w3.org/ns/shacl#>
PREFIX xsd: <http://www.w3.org/2001/XMLSchema#>
PREFIX rdfs: <http://www.w3.org/2000/01/rdf-schema#>
PREFIX MovieSHACL3: <http://example.org/ontologies/MovieSHACL3#>
PREFIX graphql: <http://datashapes.org/graphql#>
PREFIX dash: <http://datashapes.org/dash#>

<urn:x-evn-master:movieontology>
        owl:imports          <http://datashapes.org/graphql>;
        rdf:type             owl:Ontology;
        <http://topbraid.org/swa#defaultNamespace>  "http://example.org/ontologies/MovieOntology#";
        rdfs:label           "MovieSHACL";
        metadata:status      metadata:UnderDevelopmentStatus;
        graphql:publicClass  MovieSHACL3:Person;
        graphql:publicClass  MovieSHACL3:Film;
        graphql:publicClass  MovieSHACL3:Award;
        graphql:publicClass  MovieSHACL3:AwardCategory;
        graphql:publicClass  MovieSHACL3:Nomination;
        graphql:publicClass  MovieSHACL3:AwardSystem .

MovieSHACL3:Actor  rdfs:subClassOf  MovieSHACL3:Person;
        rdf:type         sh:NodeShape;
        rdf:type         owl:Class;
        rdfs:label       "Actor";
        rdfs:comment     "A person who performs a role in a movie by portraying a character.\n" .

MovieSHACL3:Person  rdfs:subClassOf  owl:Thing;
        rdf:type         sh:NodeShape;
        rdf:type         owl:Class;
        rdfs:label       "Person"@en;
        rdfs:comment     "An individual involved in the creation or production of a movie. A Person may participate in one or more roles (director, actor, producer, etc.) via relationship properties on Film. Roles are expressed through relationships, not subclasses.\n"@en;
        sh:property      MovieSHACL3:Person-fullName;
        sh:property      MovieSHACL3:Person-birthYear;
        sh:property      MovieSHACL3:Person-biography;
        sh:property      MovieSHACL3:Person-hasIdentifier;
        sh:property      MovieSHACL3:Person-label .

MovieSHACL3:Person-fullName
        rdf:type     sh:PropertyShape;
        sh:name      "fullName";
        sh:path      MovieSHACL3:fullName;
        sh:maxCount  1;
        sh:datatype  xsd:string;
        sh:minCount  1 .

MovieSHACL3:Person-birthYear
        rdf:type     sh:PropertyShape;
        sh:name      "birthYear";
        sh:path      MovieSHACL3:birthYear;
        sh:maxCount  1;
        sh:datatype  xsd:integer .

MovieSHACL3:Person-biography
        rdf:type     sh:PropertyShape;
        sh:name      "biography";
        sh:path      MovieSHACL3:biography;
        sh:maxCount  1;
        sh:datatype  xsd:string .

MovieSHACL3:Person-hasIdentifier
        rdf:type     sh:PropertyShape;
        sh:nodeKind  sh:IRI;
        sh:class     MovieSHACL3:Identifier;
        sh:name      "hasIdentifier";
        sh:path      MovieSHACL3:hasIdentifier .

MovieSHACL3:Person-label
        rdf:type       sh:PropertyShape;
        graphql:name   "labels";
        sh:name        "labels";
        sh:path        rdfs:label;
        sh:or          dash:StringOrLangString;
        sh:singleLine  true .

MovieSHACL3:tmdb  rdf:type  MovieSHACL3:IdentifierScheme;
        rdfs:label  "tmdb"@en .

MovieSHACL3:IdentifierScheme
        rdfs:subClassOf  owl:Thing;
        rdf:type         sh:NodeShape;
        rdf:type         owl:Class;
        rdfs:label       "IdentifierScheme";
        rdfs:comment     "A controlled vocabulary of identifier schemes (e.g., tmdb, imdb, wikidata).\n"@en;
        sh:property      MovieSHACL3:IdentifierScheme-label .

MovieSHACL3:Identifier-scheme
        rdf:type     sh:PropertyShape;
        sh:nodeKind  sh:IRI;
        sh:class     MovieSHACL3:IdentifierScheme;
        sh:name      "scheme";
        sh:path      MovieSHACL3:scheme;
        sh:maxCount  1;
        sh:minCount  1 .

MovieSHACL3:Nomination-yearFilm
        rdf:type     sh:PropertyShape;
        sh:name      "yearFilm";
        sh:path      MovieSHACL3:yearFilm;
        sh:maxCount  1;
        sh:datatype  xsd:gYear;
        sh:minCount  1 .

MovieSHACL3:AwardSystem
        rdfs:subClassOf  owl:Thing;
        rdf:type         sh:NodeShape;
        rdf:type         owl:Class;
        rdfs:label       "AwardSystem"@en;
        rdfs:comment     "An organized award program administered by a specific body (e.g., Academy Awards/Oscars, BAFTA, SAG, DGA, PGA). Each AwardSystem has its own set of categories and annual ceremonies.\n"@en;
        sh:property      MovieSHACL3:AwardSystem-systemName;
        sh:property      MovieSHACL3:AwardSystem-shortName;
        sh:property      MovieSHACL3:AwardSystem-description;
        sh:property      MovieSHACL3:AwardSystem-label .

MovieSHACL3:AwardSystem-systemName
        rdf:type     sh:PropertyShape;
        sh:name      "systemName";
        sh:path      MovieSHACL3:systemName;
        sh:maxCount  1;
        sh:datatype  xsd:string;
        sh:minCount  1 .

MovieSHACL3:AwardSystem-shortName
        rdf:type     sh:PropertyShape;
        sh:name      "shortName";
        sh:path      MovieSHACL3:shortName;
        sh:maxCount  1;
        sh:datatype  xsd:string;
        sh:minCount  1 .

MovieSHACL3:AwardSystem-description
        rdf:type     sh:PropertyShape;
        sh:name      "description";
        sh:path      MovieSHACL3:description;
        sh:maxCount  1;
        sh:datatype  xsd:string .

MovieSHACL3:AwardSystem-label
        rdf:type       sh:PropertyShape;
        graphql:name   "labels";
        sh:name        "labels";
        sh:path        rdfs:label;
        sh:or          dash:StringOrLangString;
        sh:singleLine  true .

MovieSHACL3:AwardCeremony
        rdfs:subClassOf  owl:Thing;
        rdf:type         sh:NodeShape;
        rdf:type         owl:Class;
        rdfs:label       "AwardCeremony";
        rdfs:comment     "An award ceremony event for a specific year (e.g., the 96th Academy Awards), typically recognizing films from a prior release year.\n"@en;
        sh:property      MovieSHACL3:AwardCeremony-yearCeremony;
        sh:property      MovieSHACL3:AwardCeremony-ceremonyName;
        sh:property      MovieSHACL3:AwardCeremony-ceremonyDate;
        sh:property      MovieSHACL3:AwardCeremony-hasAwardSystem;
        sh:property      MovieSHACL3:AwardCeremony-label .

MovieSHACL3:AwardCeremony-hasAwardSystem
        rdf:type     sh:PropertyShape;
        sh:nodeKind  sh:IRI;
        sh:class     MovieSHACL3:AwardSystem;
        sh:name      "hasAwardSystem";
        sh:path      MovieSHACL3:hasAwardSystem;
        sh:maxCount  1;
        sh:minCount  1 .

MovieSHACL3:AwardCeremony-yearCeremony
        rdf:type     sh:PropertyShape;
        sh:name      "yearCeremony";
        sh:path      MovieSHACL3:yearCeremony;
        sh:maxCount  1;
        sh:datatype  xsd:gYear;
        sh:minCount  1 .

MovieSHACL3:AwardCeremony-ceremonyName
        rdf:type     sh:PropertyShape;
        sh:name      "ceremonyName";
        sh:path      MovieSHACL3:ceremonyName;
        sh:maxCount  1;
        sh:datatype  xsd:string;
        sh:minCount  1 .

MovieSHACL3:AwardCeremony-ceremonyDate
        rdf:type     sh:PropertyShape;
        sh:name      "ceremonyDate";
        sh:path      MovieSHACL3:ceremonyDate;
        sh:maxCount  1;
        sh:datatype  xsd:date .

MovieSHACL3:AwardCeremony-label
        rdf:type       sh:PropertyShape;
        graphql:name   "labels";
        sh:name        "labels";
        sh:path        rdfs:label;
        sh:or          dash:StringOrLangString;
        sh:singleLine  true .

MovieSHACL3:Identifier-label
        rdf:type       sh:PropertyShape;
        graphql:name   "labels";
        sh:name        "labels";
        sh:path        rdfs:label;
        sh:or          dash:StringOrLangString;
        sh:singleLine  true .

MovieSHACL3:Film-label
        rdf:type       sh:PropertyShape;
        graphql:name   "labels";
        sh:name        "labels";
        sh:path        rdfs:label;
        sh:or          dash:StringOrLangString;
        sh:singleLine  true .

MovieSHACL3:Film-hasDirector
        rdf:type     sh:PropertyShape;
        sh:nodeKind  sh:IRI;
        sh:class     MovieSHACL3:Person;
        sh:name      "hasDirector";
        sh:path      MovieSHACL3:hasDirector .

MovieSHACL3:Film-hasActor
        rdf:type     sh:PropertyShape;
        sh:nodeKind  sh:IRI;
        sh:class     MovieSHACL3:Person;
        sh:name      "hasActor";
        sh:path      MovieSHACL3:hasActor .

MovieSHACL3:Film-hasProducer
        rdf:type     sh:PropertyShape;
        sh:nodeKind  sh:IRI;
        sh:class     MovieSHACL3:Person;
        sh:name      "hasProducer";
        sh:path      MovieSHACL3:hasProducer .

MovieSHACL3:Film-hasWriter
        rdf:type     sh:PropertyShape;
        sh:nodeKind  sh:IRI;
        sh:class     MovieSHACL3:Person;
        sh:name      "hasWriter";
        sh:path      MovieSHACL3:hasWriter .

MovieSHACL3:Film-hasComposer
        rdf:type     sh:PropertyShape;
        sh:nodeKind  sh:IRI;
        sh:class     MovieSHACL3:Person;
        sh:name      "hasComposer";
        sh:path      MovieSHACL3:hasComposer .

MovieSHACL3:Film-hasCinematographer
        rdf:type     sh:PropertyShape;
        sh:nodeKind  sh:IRI;
        sh:class     MovieSHACL3:Person;
        sh:name      "hasCinematographer";
        sh:path      MovieSHACL3:hasCinematographer .

MovieSHACL3:Director  rdfs:subClassOf  MovieSHACL3:Person;
        rdf:type         sh:NodeShape;
        rdf:type         owl:Class;
        rdfs:label       "Director";
        rdfs:comment     "A person responsible for overseeing the creative and artistic aspects of a movie, including directing performances and guiding the overall vision of the film.\n" .

MovieSHACL3:Nomination
        rdfs:subClassOf  owl:Thing;
        rdf:type         sh:NodeShape;
        rdf:type         owl:Class;
        rdfs:label       "Nomination"@en;
        rdfs:comment     "A reified time-bound event representing a nomination for an award category at a specific ceremony. The linked AwardCeremony provides the authoritative temporal anchor (ceremonyYear). Supports film-level (Best Picture), person-specific (Best Director), and collaboration (Best Original Song) nomination types.\n"@en;
        sh:property      MovieSHACL3:Nomination-yearFilm;
        sh:property      MovieSHACL3:Nomination-hasCeremony;
        sh:property      MovieSHACL3:Nomination-previousNominations;
        sh:property      MovieSHACL3:Nomination-winner;
        sh:property      MovieSHACL3:Nomination-hasCanonCategory;
        sh:property      MovieSHACL3:Nomination-label;
        sh:property      MovieSHACL3:Nomination-hasFilm;
        sh:property      MovieSHACL3:Nomination-hasNominee;
        sh:property      MovieSHACL3:Nomination-hasCategory;
        sh:property      MovieSHACL3:Nomination-previousWins;
        sh:property      MovieSHACL3:Nomination-nomineeType .

MovieSHACL3:Nomination-hasCeremony
        rdf:type     sh:PropertyShape;
        sh:nodeKind  sh:IRI;
        sh:class     MovieSHACL3:AwardCeremony;
        sh:name      "hasCeremony";
        sh:path      MovieSHACL3:hasCeremony;
        sh:minCount  1;
        sh:maxCount  1 .

MovieSHACL3:Nomination-previousNominations
        rdf:type          sh:PropertyShape;
        sh:name           "previousNominations";
        sh:path           MovieSHACL3:previousNominations;
        sh:maxCount       1;
        sh:datatype       xsd:integer;
        sh:minInclusive   0 .

MovieSHACL3:Nomination-winner
        rdf:type     sh:PropertyShape;
        sh:name      "winner";
        sh:path      MovieSHACL3:winner;
        sh:maxCount  1;
        sh:datatype  xsd:boolean;
        sh:minCount  1 .

MovieSHACL3:Nomination-hasCanonCategory
        rdf:type     sh:PropertyShape;
        sh:nodeKind  sh:IRI;
        sh:class     MovieSHACL3:AwardCategory;
        sh:name      "hasCanonCategory";
        sh:path      MovieSHACL3:hasCanonCategory;
        sh:maxCount  1 .

MovieSHACL3:Nomination-label
        rdf:type       sh:PropertyShape;
        graphql:name   "labels";
        sh:name        "labels";
        sh:path        rdfs:label;
        sh:or          dash:StringOrLangString;
        sh:singleLine  true .

MovieSHACL3:Nomination-hasFilm
        rdf:type     sh:PropertyShape;
        sh:nodeKind  sh:IRI;
        sh:class     MovieSHACL3:Film;
        sh:name      "hasFilm";
        sh:path      MovieSHACL3:hasFilm;
        sh:maxCount  1 .

MovieSHACL3:Nomination-hasNominee
        rdf:type     sh:PropertyShape;
        sh:nodeKind  sh:IRI;
        sh:class     MovieSHACL3:Person;
        sh:name      "hasNominee";
        sh:path      MovieSHACL3:hasNominee .

MovieSHACL3:Nomination-hasCategory
        rdf:type     sh:PropertyShape;
        sh:nodeKind  sh:IRI;
        sh:class     MovieSHACL3:AwardCategory;
        sh:name      "hasCategory";
        sh:path      MovieSHACL3:hasCategory;
        sh:minCount  1;
        sh:maxCount  1 .

MovieSHACL3:Nomination-previousWins
        rdf:type          sh:PropertyShape;
        sh:name           "previousWins";
        sh:path           MovieSHACL3:previousWins;
        sh:maxCount       1;
        sh:datatype       xsd:integer;
        sh:minInclusive   0 .

MovieSHACL3:Nomination-nomineeType
        rdf:type     sh:PropertyShape;
        sh:name      "nomineeType";
        sh:path      MovieSHACL3:nomineeType;
        sh:maxCount  1;
        sh:datatype  xsd:string;
        sh:in        ( "FILM" "PERSON" "COLLABORATION" ) .

MovieSHACL3:Award-label
        rdf:type       sh:PropertyShape;
        graphql:name   "labels";
        sh:name        "labels";
        sh:path        rdfs:label;
        sh:or          dash:StringOrLangString;
        sh:singleLine  true .

MovieSHACL3:Film
        rdfs:subClassOf  owl:Thing;
        rdf:type         sh:NodeShape;
        rdf:type         owl:Class;
        rdfs:label       "Film"@en;
        rdfs:comment     "A motion picture or film released to the public. Represents a completed creative work and may be associated with people (such as directors and actors), genres, release information, and awards.\n"@en;
        sh:property      MovieSHACL3:Film-label;
        sh:property      MovieSHACL3:Film-hasDirector;
        sh:property      MovieSHACL3:Film-hasActor;
        sh:property      MovieSHACL3:Film-hasProducer;
        sh:property      MovieSHACL3:Film-hasWriter;
        sh:property      MovieSHACL3:Film-hasComposer;
        sh:property      MovieSHACL3:Film-hasCinematographer;
        sh:property      MovieSHACL3:Film-hasNomination;
        sh:property      MovieSHACL3:Film-hasIdentifier;
        sh:property      MovieSHACL3:Film-wikidataId;
        sh:property      MovieSHACL3:Film-title;
        sh:property      MovieSHACL3:Film-releaseYear;
        sh:property      MovieSHACL3:Film-tmdbId;
        sh:property      MovieSHACL3:Film-imdbId;
        sh:property      MovieSHACL3:Film-runtime;
        sh:property      MovieSHACL3:Film-genre;
        sh:property      MovieSHACL3:Film-language;
        sh:property      MovieSHACL3:Film-country;
        sh:property      MovieSHACL3:Film-productionCompany;
        sh:property      MovieSHACL3:Film-budget;
        sh:property      MovieSHACL3:Film-boxOffice;
        sh:property      MovieSHACL3:Film-synopsis .

MovieSHACL3:AwardCategory-label
        rdf:type       sh:PropertyShape;
        graphql:name   "labels";
        sh:name        "labels";
        sh:path        rdfs:label;
        sh:or          dash:StringOrLangString;
        sh:singleLine  true .

MovieSHACL3:Identifier
        rdfs:subClassOf  owl:Thing;
        rdf:type         sh:NodeShape;
        rdf:type         owl:Class;
        rdfs:label       "Identifier";
        rdfs:comment     "An external identifier for a Person or Movie (e.g., TMDB, IMDb, Wikidata).\n"@en;
        sh:property      MovieSHACL3:Identifier-scheme;
        sh:property      MovieSHACL3:Identifier-label;
        sh:property      MovieSHACL3:Identifier-value .

MovieSHACL3:Identifier-value
        rdf:type     sh:PropertyShape;
        sh:name      "value";
        sh:path      MovieSHACL3:value;
        sh:maxCount  1;
        sh:datatype  xsd:string;
        sh:minCount  1 .

MovieSHACL3:Award  rdfs:subClassOf  owl:Thing;
        rdf:type         sh:NodeShape;
        rdf:type         owl:Class;
        rdfs:label       "Award";
        rdfs:comment     "A recognition or honor bestowed on a movie or person for achievement in filmmaking, typically granted by an awarding body or organization.\n";
        sh:property      MovieSHACL3:Award-label .

MovieSHACL3:IdentifierScheme-label
        rdf:type       sh:PropertyShape;
        graphql:name   "labels";
        sh:name        "labels";
        sh:path        rdfs:label;
        sh:or          dash:StringOrLangString;
        sh:singleLine  true .

MovieSHACL3:Film-hasIdentifier
        rdf:type     sh:PropertyShape;
        sh:nodeKind  sh:IRI;
        sh:class     MovieSHACL3:Identifier;
        sh:name      "hasIdentifier";
        sh:path      MovieSHACL3:hasIdentifier .

MovieSHACL3:Film-hasNomination
        rdf:type     sh:PropertyShape;
        sh:nodeKind  sh:IRI;
        sh:class     MovieSHACL3:Nomination;
        sh:name      "hasNomination";
        sh:path      MovieSHACL3:hasNomination .

MovieSHACL3:Film-wikidataId
        rdf:type     sh:PropertyShape;
        sh:name      "wikidataId";
        sh:path      MovieSHACL3:wikidataId;
        sh:maxCount  1;
        sh:datatype  xsd:string .

MovieSHACL3:imdb  rdf:type  MovieSHACL3:IdentifierScheme;
        rdfs:label  "imdb"@en .

MovieSHACL3:Film-title
        rdf:type     sh:PropertyShape;
        sh:name      "title";
        sh:path      MovieSHACL3:title;
        sh:maxCount  1;
        sh:datatype  xsd:string;
        sh:minCount  1 .

MovieSHACL3:Film-releaseYear
        rdf:type     sh:PropertyShape;
        sh:name      "releaseYear";
        sh:path      MovieSHACL3:releaseYear;
        sh:maxCount  1;
        sh:datatype  xsd:gYear;
        sh:minCount  1 .

MovieSHACL3:AwardCategory
        rdfs:subClassOf  owl:Thing;
        rdf:type         sh:NodeShape;
        rdf:type         owl:Class;
        rdfs:label       "AwardCategory";
        rdfs:comment     "A specific award category within an award system (e.g., Best Picture for Oscars, Best Film for BAFTA). Categories are system-specific and not normalized across systems in Phase 1.\n"@en;
        sh:property      MovieSHACL3:AwardCategory-categoryName;
        sh:property      MovieSHACL3:AwardCategory-label;
        sh:property      MovieSHACL3:AwardCategory-hasAwardSystem;
        sh:property      MovieSHACL3:AwardCategory-description .

MovieSHACL3:AwardCategory-categoryName
        rdf:type     sh:PropertyShape;
        sh:name      "categoryName";
        sh:path      MovieSHACL3:categoryName;
        sh:maxCount  1;
        sh:datatype  xsd:string;
        sh:minCount  1 .

MovieSHACL3:AwardCategory-hasAwardSystem
        rdf:type     sh:PropertyShape;
        sh:nodeKind  sh:IRI;
        sh:class     MovieSHACL3:AwardSystem;
        sh:name      "hasAwardSystem";
        sh:path      MovieSHACL3:hasAwardSystem;
        sh:maxCount  1;
        sh:minCount  1 .

MovieSHACL3:AwardCategory-description
        rdf:type     sh:PropertyShape;
        sh:name      "description";
        sh:path      MovieSHACL3:description;
        sh:maxCount  1;
        sh:datatype  xsd:string .

MovieSHACL3:Film-tmdbId
        rdf:type     sh:PropertyShape;
        sh:name      "tmdbId";
        sh:path      MovieSHACL3:tmdbId;
        sh:maxCount  1;
        sh:datatype  xsd:string .

MovieSHACL3:wikidata  rdf:type  MovieSHACL3:IdentifierScheme;
        rdfs:label  "wikidata"@en .

MovieSHACL3:Genre  rdfs:subClassOf  owl:Thing;
        rdf:type         sh:NodeShape;
        rdf:type         owl:Class;
        rdfs:label       "Genre";
        rdfs:comment     "A category used to classify movies based on shared thematic, narrative, or stylistic characteristics, such as Drama, Comedy, or Science Fiction.\n" .

MovieSHACL3:Film-imdbId
        rdf:type       sh:PropertyShape;
        sh:name        "imdbId";
        sh:path        MovieSHACL3:imdbId;
        sh:maxCount    1;
        sh:datatype    xsd:string;
        dash:uriStart  "example.org/movie-" .

MovieSHACL3:Film-runtime
        rdf:type          sh:PropertyShape;
        sh:name           "runtime";
        sh:path           MovieSHACL3:runtime;
        sh:maxCount       1;
        sh:datatype       xsd:integer;
        sh:minInclusive   1 .

MovieSHACL3:Film-genre
        rdf:type     sh:PropertyShape;
        sh:nodeKind  sh:IRI;
        sh:class     MovieSHACL3:Genre;
        sh:name      "hasGenre";
        sh:path      MovieSHACL3:hasGenre .

MovieSHACL3:Film-language
        rdf:type     sh:PropertyShape;
        sh:name      "language";
        sh:path      MovieSHACL3:language;
        sh:maxCount  1;
        sh:datatype  xsd:string .

MovieSHACL3:Film-country
        rdf:type     sh:PropertyShape;
        sh:name      "country";
        sh:path      MovieSHACL3:country;
        sh:datatype  xsd:string .

MovieSHACL3:Film-productionCompany
        rdf:type     sh:PropertyShape;
        sh:name      "productionCompany";
        sh:path      MovieSHACL3:productionCompany;
        sh:datatype  xsd:string .

MovieSHACL3:Film-budget
        rdf:type          sh:PropertyShape;
        sh:name           "budget";
        sh:path           MovieSHACL3:budget;
        sh:maxCount       1;
        sh:datatype       xsd:decimal;
        sh:minInclusive   0 .

MovieSHACL3:Film-boxOffice
        rdf:type          sh:PropertyShape;
        sh:name           "boxOffice";
        sh:path           MovieSHACL3:boxOffice;
        sh:maxCount       1;
        sh:datatype       xsd:decimal;
        sh:minInclusive   0 .

MovieSHACL3:Film-synopsis
        rdf:type     sh:PropertyShape;
        sh:name      "synopsis";
        sh:path      MovieSHACL3:synopsis;
        sh:maxCount  1;
        sh:datatype  xsd:string .
